lakefile.lean
@@ -4,8 +4,7 @@ open Lake DSL
 package «verity-benchmark» where
   version := v!"0.1.0"
 
-require verity from git
-  "https://github.com/lfglabs-dev/verity.git"@"03447eab62ef41d34535170a88c97e2a9d9715cc"
+require verity from git "https://github.com/lfglabs-dev/verity.git"@"7ac455b22bf56c32245c35470abeaba03e3c88b7"
 
 @[default_target]
 lean_lib «Benchmark» where
